Refactor parameters of properties
In the properties, determine parameters like the set of invoked
capabilities from the trace (using functions provided by the ISA
instantiation) rather than passing them in using a large number of
arguments;  this should simplify adding more parameters.

model/isabelle/Cheri_axioms_lemmas.thy
@@ -7,8 +7,20 @@ locale Capability_ISA = Capabilities CC
   fixes ISA :: "('cap, 'regval, 'instr, 'e) isa"
     and initial_caps :: "'cap set"
 
+abbreviation "instr_trace instr t \<equiv> \<lparr>trace = t, trace_kind = Instr_Trace instr\<rparr>"
+abbreviation "fetch_trace t \<equiv> \<lparr>trace = t, trace_kind = Fetch_Trace\<rparr>"
+
+lemma trace_invokes_simps[simp]:
+  "trace_invokes_caps ISA (instr_trace instr t) = instr_invokes_caps ISA instr t"
+  "trace_invokes_caps ISA (fetch_trace t) = {}"
+  "trace_invokes_indirect_caps ISA (instr_trace instr t) = instr_invokes_indirect_caps ISA instr t"
+  "trace_invokes_indirect_caps ISA (fetch_trace t) = {}"
+  by (auto simp: trace_invokes_caps_def trace_invokes_indirect_caps_def)
+
+declare event_at_idx_def[simp]
+
 lemma reads_from_reg_at_idx_Some_iff[simp]:
-  "reads_from_reg_at_idx i t = Some r \<longleftrightarrow> reads_from_reg (t ! i) = Some r \<and> i < length t"
+  "reads_from_reg_at_idx i t = Some r \<longleftrightarrow> reads_from_reg (trace t ! i) = Some r \<and> i < length (trace t)"
   by (auto simp: reads_from_reg_at_idx_def bind_eq_Some_conv)
 
 lemma reads_from_reg_SomeE[elim!]:
@@ -23,7 +35,7 @@ lemma reads_from_reg_Some_iff:
 
 lemma member_reads_reg_caps_at_idx_iff[simp]:
   "c \<in> reads_reg_caps_at_idx CC ISA i t \<longleftrightarrow>
-   c \<in> reads_reg_caps CC (caps_of_regval ISA) (t ! i) \<and> i < length t"
+   c \<in> reads_reg_caps CC (caps_of_regval ISA) (trace t ! i) \<and> i < length (trace t)"
   by (auto simp: reads_reg_caps_at_idx_def split: option.splits)
 
 lemma member_reads_reg_caps_iff:
@@ -43,7 +55,7 @@ lemma reads_reg_caps_Some_reads_mem_cap_None[simp]:
   using assms by (cases e) (auto simp: reads_mem_cap_def)
 
 lemma writes_to_reg_at_idx_Some_iff[simp]:
-  "writes_to_reg_at_idx i t = Some r \<longleftrightarrow> writes_to_reg (t ! i) = Some r \<and> i < length t"
+  "writes_to_reg_at_idx i t = Some r \<longleftrightarrow> writes_to_reg (trace t ! i) = Some r \<and> i < length (trace t)"
   by (auto simp: writes_to_reg_at_idx_def bind_eq_Some_conv)
 
 lemma writes_to_reg_SomeE[elim!]:
@@ -58,7 +70,7 @@ lemma writes_to_reg_Some_iff:
 
 lemma member_writes_reg_caps_at_idx_iff[simp]:
   "c \<in> writes_reg_caps_at_idx CC ISA i t \<longleftrightarrow>
-   c \<in> writes_reg_caps CC (caps_of_regval ISA) (t ! i) \<and> i < length t"
+   c \<in> writes_reg_caps CC (caps_of_regval ISA) (trace t ! i) \<and> i < length (trace t)"
   by (auto simp: writes_reg_caps_at_idx_def split: option.splits)
 
 lemma member_writes_reg_capsE[elim!]:
@@ -74,12 +86,12 @@ lemma member_writes_reg_caps_iff:
 
 lemma writes_mem_cap_at_idx_Some_iff[simp]:
   "writes_mem_cap_at_idx CC i t = Some (addr, sz, c) \<longleftrightarrow>
-   writes_mem_cap CC (t ! i) = Some (addr, sz, c) \<and> i < length t"
+   writes_mem_cap CC (trace t ! i) = Some (addr, sz, c) \<and> i < length (trace t)"
   by (auto simp: writes_mem_cap_at_idx_def bind_eq_Some_conv)
 
 lemma reads_mem_cap_at_idx_Some_iff[simp]:
   "reads_mem_cap_at_idx CC i t = Some (addr, sz, c) \<longleftrightarrow>
-   reads_mem_cap CC (t ! i) = Some (addr, sz, c) \<and> i < length t"
+   reads_mem_cap CC (trace t ! i) = Some (addr, sz, c) \<and> i < length (trace t)"
   by (auto simp: reads_mem_cap_at_idx_def bind_eq_Some_conv)
 
 lemma nth_append_left:
@@ -116,9 +128,9 @@ lemma reads_mem_cap_Some_iff:
 
 lemma available_reg_capsE:
   assumes "c \<in> available_reg_caps CC ISA i t"
-  obtains r v j where "t ! j = E_read_reg r v"
+  obtains r v j where "trace t ! j = E_read_reg r v"
     and "c \<in> caps_of_regval ISA v" and "is_tagged_method CC c"
-    and "j < length t" and "j < i"
+    and "j < length (trace t)" and "j < i"
     and "r \<in> PCC ISA \<or> r \<in> IDC ISA \<longrightarrow> \<not>cap_reg_written_before_idx CC ISA j r t"
     and "r \<in> read_privileged_regs ISA \<longrightarrow> system_access_permitted_before_idx CC ISA j t"
   using assms
@@ -126,25 +138,25 @@ lemma available_reg_capsE:
 
 lemma available_mem_capsE:
   assumes "c \<in> available_mem_caps CC ISA i t"
-  obtains wk paddr bytes j sz where "t ! j = E_read_memt wk paddr sz (bytes, B1)"
-    and "\<not>is_translation_event ISA (t ! j)"
+  obtains wk paddr bytes j sz where "trace t ! j = E_read_memt wk paddr sz (bytes, B1)"
+    and "\<not>is_translation_event ISA (trace t ! j)"
     and "cap_of_mem_bytes_method CC bytes B1 = Some c"
-    and "j < i" and "j < length t" and "is_tagged_method CC c"
+    and "j < i" and "j < length (trace t)" and "is_tagged_method CC c"
   using assms
   by (induction i) (auto split: option.splits if_splits)
 
 lemma available_caps_cases:
-  assumes "c \<in> available_caps CC ISA use_mem_caps i t"
-  obtains (Reg) r v j where "t ! j = E_read_reg r v"
+  assumes "c \<in> available_caps CC ISA i t"
+  obtains (Reg) r v j where "trace t ! j = E_read_reg r v"
     and "c \<in> caps_of_regval ISA v" and "is_tagged_method CC c"
-    and "j < length t" and "j < i"
+    and "j < length (trace t)" and "j < i"
     and "r \<in> PCC ISA \<or> r \<in> IDC ISA \<longrightarrow> \<not>cap_reg_written_before_idx CC ISA j r t"
     and "r \<in> read_privileged_regs ISA \<longrightarrow> system_access_permitted_before_idx CC ISA j t"
-  | (Mem) wk paddr bytes j sz where "t ! j = E_read_memt wk paddr sz (bytes, B1)"
-    and "\<not>is_translation_event ISA (t ! j)"
+  | (Mem) wk paddr bytes j sz where "trace t ! j = E_read_memt wk paddr sz (bytes, B1)"
+    and "\<not>is_translation_event ISA (trace t ! j)"
     and "cap_of_mem_bytes_method CC bytes B1 = Some c"
-    and "j < i" and "j < length t" and "is_tagged_method CC c"
-    and "use_mem_caps"
+    and "j < i" and "j < length (trace t)" and "is_tagged_method CC c"
+    and "trace_uses_mem_caps ISA t" and "trace_invokes_indirect_caps ISA t = {}"
   using assms
   unfolding available_caps_def
   by (fastforce split: if_splits elim: available_reg_capsE available_mem_capsE)
@@ -156,10 +168,10 @@ lemma cap_reg_written_before_idx_0_False[simp]:
 lemma cap_reg_written_before_idx_Suc_iff[simp]:
   "cap_reg_written_before_idx CC ISA (Suc i) r t \<longleftrightarrow>
    (cap_reg_written_before_idx CC ISA i r t \<or>
-    (\<exists>v c. i < length t \<and> t ! i = E_write_reg r v \<and> c \<in> caps_of_regval ISA v \<and> is_tagged_method CC c))"
+    (\<exists>v c. i < length (trace t) \<and> trace t ! i = E_write_reg r v \<and> c \<in> caps_of_regval ISA v \<and> is_tagged_method CC c))"
   by (fastforce simp: cap_reg_written_before_idx_def less_Suc_eq)
 
-definition accessible_regs_at_idx :: "nat \<Rightarrow> 'regval trace \<Rightarrow> register_name set" where
+definition accessible_regs_at_idx :: "nat \<Rightarrow> ('regval, 'instr) isa_trace \<Rightarrow> register_name set" where
   "accessible_regs_at_idx i t =
      {r. (r \<in> PCC ISA \<or> r \<in> IDC ISA \<longrightarrow> \<not>cap_reg_written_before_idx CC ISA i r t) \<and>
          (r \<in> read_privileged_regs ISA \<longrightarrow> system_access_permitted_before_idx CC ISA i t)}"
@@ -206,7 +218,7 @@ lemma system_access_permitted_before_idx_0[simp]:
 lemma system_access_permitted_before_idx_Suc[simp]:
   "system_access_permitted_before_idx CC ISA (Suc i) t \<longleftrightarrow>
      (system_access_permitted_before_idx CC ISA i t \<or>
-      (i < length t \<and> allows_system_reg_access (accessible_regs_at_idx i t) (t ! i)))"
+      (i < length (trace t) \<and> allows_system_reg_access (accessible_regs_at_idx i t) (trace t ! i)))"
   by (fastforce simp: system_access_permitted_before_idx_def accessible_regs_at_idx_def less_Suc_eq
                 elim!: allows_system_reg_access.elims)
 
@@ -217,9 +229,9 @@ lemma accessible_regs_at_idx_0[simp]:
 lemma accessible_regs_at_idx_Suc:
   "accessible_regs_at_idx (Suc i) t =
      (accessible_regs_at_idx i t \<union>
-     (if i < length t \<and> allows_system_reg_access (accessible_regs_at_idx i t) (t ! i)
+     (if i < length (trace t) \<and> allows_system_reg_access (accessible_regs_at_idx i t) (trace t ! i)
       then {r \<in> read_privileged_regs ISA. r \<in> PCC ISA \<or> r \<in> IDC ISA \<longrightarrow> \<not>cap_reg_written_before_idx CC ISA i r t} else {})) -
-     {r \<in> PCC ISA \<union> IDC ISA. \<exists>c v. i < length t \<and> t ! i = E_write_reg r v \<and> c \<in> caps_of_regval ISA v \<and> is_tagged_method CC c}"
+     {r \<in> PCC ISA \<union> IDC ISA. \<exists>c v. i < length (trace t) \<and> trace t ! i = E_write_reg r v \<and> c \<in> caps_of_regval ISA v \<and> is_tagged_method CC c}"
   by (auto simp: accessible_regs_at_idx_def)
 
 lemma reads_from_reg_None_reads_reg_caps_empty[simp]:
@@ -235,42 +247,42 @@ lemma available_reg_caps_0[simp]: "available_reg_caps CC ISA 0 t = {}"
 lemma available_mem_caps_0[simp]: "available_mem_caps CC ISA 0 t = {}"
   by (auto simp: available_mem_caps.simps)
 
-lemma available_caps_0[simp]: "available_caps CC ISA use_mem_caps 0 t = {}"
+lemma available_caps_0[simp]: "available_caps CC ISA 0 t = {}"
   by (auto simp: available_caps_def)
 
 lemma available_reg_caps_Suc:
   "available_reg_caps CC ISA (Suc i) t =
      available_reg_caps CC ISA i t
-     \<union> (if i < length t then accessed_reg_caps_of_ev (accessible_regs_at_idx i t) (t ! i) else {})"
-  by (cases "t ! i") (auto simp: available_reg_caps.simps accessible_regs_at_idx_def)
+     \<union> (if i < length (trace t) then accessed_reg_caps_of_ev (accessible_regs_at_idx i t) (trace t ! i) else {})"
+  by (cases "trace t ! i") (auto simp: available_reg_caps.simps accessible_regs_at_idx_def)
 
 lemma available_mem_caps_Suc:
   "available_mem_caps CC ISA (Suc i) t =
      available_mem_caps CC ISA i t
-     \<union> (if i < length t then accessed_mem_caps_of_ev (t ! i) else {})"
-  by (cases "t ! i")
+     \<union> (if i < length (trace t) then accessed_mem_caps_of_ev (trace t ! i) else {})"
+  by (cases "trace t ! i")
      (auto simp: available_mem_caps.simps reads_mem_cap_def bind_eq_Some_conv split: option.splits)
 
 lemma available_caps_Suc:
-  "available_caps CC ISA use_mem_caps (Suc i) t =
-   available_caps CC ISA use_mem_caps i t \<union>
-   (if i < length t then accessed_reg_caps_of_ev (accessible_regs_at_idx i t) (t ! i) else {}) \<union>
-   (if i < length t \<and> use_mem_caps then accessed_mem_caps_of_ev (t ! i) else {})"
+  "available_caps CC ISA (Suc i) t =
+   available_caps CC ISA i t \<union>
+   (if i < length (trace t) then accessed_reg_caps_of_ev (accessible_regs_at_idx i t) (trace t ! i) else {}) \<union>
+   (if i < length (trace t) \<and> trace_uses_mem_caps ISA t \<and> trace_invokes_indirect_caps ISA t = {} then accessed_mem_caps_of_ev (trace t ! i) else {})"
   by (auto simp: available_caps_def available_reg_caps_Suc available_mem_caps_Suc)
 
-lemma writes_reg_caps_at_idx_take[simp]:
+(*lemma writes_reg_caps_at_idx_take[simp]:
   assumes "i < n"
   shows "writes_reg_caps_at_idx CC ISA i (take n t) = writes_reg_caps_at_idx CC ISA i t"
     and "cap_reg_written_before_idx CC ISA i r (take n t) = cap_reg_written_before_idx CC ISA i r t"
   using assms
   unfolding cap_reg_written_before_idx_def writes_reg_caps_at_idx_def
-  by (auto simp: not_le split: option.splits)
+  by (auto simp: not_le split: option.splits)*)
 
-abbreviation "instr_cheri_axioms instr t n \<equiv> cheri_axioms CC ISA False (instr_raises_ex ISA instr t) initial_caps (uses_mem_caps ISA instr t) (invokes_caps ISA instr t) (invokes_indirect_caps ISA instr t) (take n t)"
+abbreviation "instr_cheri_axioms instr t n \<equiv> cheri_axioms CC ISA initial_caps n (instr_trace instr t)"
 
-abbreviation "fetch_cheri_axioms t n \<equiv> cheri_axioms CC ISA True (fetch_raises_ex ISA t) initial_caps True {} {} (take n t)"
+abbreviation "fetch_cheri_axioms t n \<equiv> cheri_axioms CC ISA initial_caps n (fetch_trace t)"
 
-lemma accessible_regs_at_idx_take[simp]:
+(*lemma accessible_regs_at_idx_take[simp]:
   "i \<le> n \<Longrightarrow> accessible_regs_at_idx i (take n t) = accessible_regs_at_idx i t"
   by (induction i) (auto simp: accessible_regs_at_idx_Suc)
 
@@ -317,14 +329,14 @@ lemma store_mem_axiom_take:
   shows "store_mem_axiom CC ISA initial_caps use_mem_caps inv_indirect_caps (take n t)"
   using assms
   unfolding store_mem_axiom_def
-  by (auto simp: writes_mem_val_at_idx_def bind_eq_Some_conv translation_event_at_idx_def min_absorb1)
+  by (auto simp: writes_mem_val_at_idx_def bind_eq_Some_conv translation_event_at_idx_def min_absorb1)*)
 
 lemma writes_mem_val_at_idx_eq_Some_iff[simp]:
   "writes_mem_val_at_idx i t = Some (addr, sz, v, tag) \<longleftrightarrow>
-   i < length t \<and> writes_mem_val (t ! i) = Some (addr, sz, v, tag)"
+   i < length (trace t) \<and> writes_mem_val (trace t ! i) = Some (addr, sz, v, tag)"
   by (auto simp: writes_mem_val_at_idx_def bind_eq_Some_conv)
 
-lemma cheri_axioms_take:
+(*lemma cheri_axioms_take:
   assumes "cheri_axioms CC ISA is_fetch has_ex initial_caps use_mem_caps inv_caps inv_indirect_caps t"
   shows "cheri_axioms CC ISA is_fetch has_ex initial_caps use_mem_caps inv_caps inv_indirect_caps (take n t)"
   using assms
@@ -335,52 +347,54 @@ lemma cheri_axioms_appendE:
   assumes "cheri_axioms CC ISA is_fetch has_ex initial_caps use_mem_caps inv_caps inv_indirect_caps (t1 @ t2)"
   shows "cheri_axioms CC ISA is_fetch has_ex initial_caps use_mem_caps inv_caps inv_indirect_caps t1"
   using cheri_axioms_take[OF assms, where n = "length t1"]
-  by simp
+  by simp*)
 
 abbreviation instr_sem_ISA ("\<lbrakk>_\<rbrakk>") where "\<lbrakk>instr\<rbrakk> \<equiv> instr_sem ISA instr"
 
 end
 
 lemma load_mem_axiomE:
-  assumes "load_mem_axiom CC ISA is_fetch initial_caps use_mem_caps invoked_indirect_caps t"
+  assumes "load_mem_axiom CC ISA initial_caps n t"
     and "reads_mem_val_at_idx i t = Some (paddr, sz, v, tag)"
     and "\<not>translation_event_at_idx ISA i t"
+    and "i < n"
   obtains c' vaddr
-  where "cap_derivable CC (initial_caps \<union> available_caps CC ISA (invoked_indirect_caps = {} \<and> use_mem_caps) i t) c'"
+  where "cap_derivable CC (initial_caps \<union> available_caps CC ISA i t) c'"
     and "is_tagged_method CC c'"
-    and "is_sealed_method CC c' \<longrightarrow> is_indirect_sentry_method CC c' \<and> unseal_method CC c' \<in> invoked_indirect_caps"
-    and "translate_address ISA vaddr (if is_fetch then Fetch else Load) (take i t) = Some paddr"
+    and "is_sealed_method CC c' \<longrightarrow> is_indirect_sentry_method CC c' \<and> unseal_method CC c' \<in> trace_invokes_indirect_caps ISA t"
+    and "translate_address ISA vaddr (if is_fetch_trace t then Fetch else Load) (take i (trace t)) = Some paddr"
     and "set (address_range vaddr sz) \<subseteq> get_mem_region CC c'"
-    and "if is_fetch then permits_execute_method CC c' else permits_load_method CC c'"
-    and "is_fetch \<longrightarrow> tag = B0"
-    and "tag \<noteq> B0 \<and> use_mem_caps \<longrightarrow> permits_load_cap_method CC c' \<and> sz = tag_granule ISA \<and> address_tag_aligned ISA paddr"
+    and "if is_fetch_trace t then permits_execute_method CC c' else permits_load_method CC c'"
+    and "is_fetch_trace t \<longrightarrow> tag = B0"
+    and "tag \<noteq> B0 \<and> trace_uses_mem_caps ISA t \<longrightarrow> permits_load_cap_method CC c' \<and> sz = tag_granule ISA \<and> address_tag_aligned ISA paddr"
   using assms
   unfolding load_mem_axiom_def
   by blast
 
 lemma store_cap_reg_axiomE:
-  assumes "store_cap_reg_axiom CC ISA has_ex initial_caps use_mem_caps invoked_caps invoked_indirect_caps t"
+  assumes "store_cap_reg_axiom CC ISA initial_caps n t"
     and "writes_to_reg_at_idx i t = Some r"
     and "c \<in> writes_reg_caps_at_idx CC ISA i t"
-  obtains (Derivable) "cap_derivable CC (initial_caps \<union> available_caps CC ISA (invoked_indirect_caps = {} \<and> use_mem_caps) i t) c"
-  | (Ex) has_ex and "r \<in> PCC ISA"
+    and "i < n"
+  obtains (Derivable) "cap_derivable CC (initial_caps \<union> available_caps CC ISA i t) c"
+  | (Ex) "trace_raises_ex ISA t" and "r \<in> PCC ISA"
     and "c \<in>  exception_targets_at_idx ISA i t"
-  | (Sentry) cs where "c \<in> invoked_caps"
-    and "cap_derivable CC (initial_caps \<union> available_caps CC ISA (invoked_indirect_caps = {} \<and> use_mem_caps) i t) cs"
+  | (Sentry) cs where "c \<in> trace_invokes_caps ISA t"
+    and "cap_derivable CC (initial_caps \<union> available_caps CC ISA i t) cs"
     and "is_sentry_method CC cs" and "is_sealed_method CC cs"
     and "leq_cap CC c (unseal_method CC cs)" and "r \<in> PCC ISA"
-  | (IndirectSentry) cs where "c \<in> invoked_indirect_caps"
+  | (IndirectSentry) cs where "c \<in> trace_invokes_indirect_caps ISA t"
     and "cap_derivable CC (initial_caps \<union> available_reg_caps CC ISA i t) cs"
     and "is_indirect_sentry_method CC cs" and "is_sealed_method CC cs"
     and "leq_cap CC c (unseal_method CC cs)" and "r \<in> IDC ISA"
-  | (CCall) cc cd where "c \<in> invoked_caps"
-    and "cap_derivable CC (initial_caps \<union> available_caps CC ISA (invoked_indirect_caps = {} \<and> use_mem_caps) i t) cc"
-    and "cap_derivable CC (initial_caps \<union> available_caps CC ISA (invoked_indirect_caps = {} \<and> use_mem_caps) i t) cd"
+  | (CCall) cc cd where "c \<in> trace_invokes_caps ISA t"
+    and "cap_derivable CC (initial_caps \<union> available_caps CC ISA i t) cc"
+    and "cap_derivable CC (initial_caps \<union> available_caps CC ISA i t) cd"
     and "invokable CC cc cd"
     and "(leq_cap CC c (unseal_method CC cc) \<and> r \<in> PCC ISA) \<or> (leq_cap CC c (unseal_method CC cd) \<and> r \<in> IDC ISA)"
-  | (Indirect) c' where "c \<in> invoked_caps"
+  | (Indirect) c' where "c \<in> trace_invokes_caps ISA t"
     and "cap_derivable CC (initial_caps \<union> available_mem_caps CC ISA i t) c'"
-    and "invoked_indirect_caps \<noteq> {}" and "use_mem_caps"
+    and "trace_invokes_indirect_caps ISA t\<noteq> {}" and "trace_uses_mem_caps ISA t"
     and "(leq_cap CC c (unseal_method CC c') \<and> is_sealed_method CC c' \<and> is_sentry_method CC c' \<and> r \<in> PCC ISA) \<or>
          (leq_cap CC c c' \<and> r \<in> PCC ISA \<union> IDC ISA)"
   using assms
@@ -414,20 +428,20 @@ fun cap_inv_ev :: "'regval event \<Rightarrow> bool" where
 
 abbreviation "cap_inv_trace t \<equiv> (\<forall>e \<in> set t. cap_inv_ev e)"
 
-definition available_caps_invariant :: "bool \<Rightarrow> 'regval event list \<Rightarrow> nat \<Rightarrow> bool" where
-  "available_caps_invariant use_mem_caps t n \<equiv>
-   (\<forall>i < n. \<forall>c \<in> initial_caps \<union> available_caps CC ISA use_mem_caps i t.
+definition available_caps_invariant :: "('regval, 'instr) isa_trace \<Rightarrow> nat \<Rightarrow> bool" where
+  "available_caps_invariant t n \<equiv>
+   (\<forall>i < n. \<forall>c \<in> initial_caps \<union> available_caps CC ISA i t.
       is_tagged_method CC c \<longrightarrow> cap_invariant c)"
 
-abbreviation
+(*abbreviation
   "instr_available_caps instr n t \<equiv>
-   available_caps CC ISA (invokes_indirect_caps ISA instr t = {} \<and> uses_mem_caps ISA instr t) n t"
+   available_caps CC ISA (invokes_indirect_caps ISA instr t = {} \<and> uses_mem_caps ISA instr t) n t"*)
 
 abbreviation
   "instr_available_caps_invariant instr t n \<equiv>
-   available_caps_invariant (invokes_indirect_caps ISA instr t = {} \<and> uses_mem_caps ISA instr t) t n"
+   available_caps_invariant (instr_trace instr t) n"
 
-abbreviation "fetch_available_caps_invariant t n \<equiv> available_caps_invariant True t n"
+abbreviation "fetch_available_caps_invariant t n \<equiv> available_caps_invariant (fetch_trace t) n"
 
 end
 
